UpdateAggregationChallenge

src/specs/UpdateAggregationChallenge.ec
@@ -1,35 +1,32 @@
 require        Constants.
+require import PointMulAndAddIntoDest.
 require import PurePrimops.
 require import UInt256.
 require import Verifier.
 require import YulPrimops.
 
 module UpdateAggregationChallenge = {
-  proc low(usr_queriesCommitmentPoint : uint256, usr_valueAtZ : uint256, usr_curAggregationChallenge : uint256, usr_curAggregatedOpeningAtZ : uint256): (uint256 * uint256) = {
-    var usr_newAggregationChallenge, usr_newAggregatedOpeningAtZ, _1, _2, _3, tmp370, _4, tmp371, _5, tmp372, _6;
-    _1 <- (W256.of_int 21888242871839275222246405745257275088548364400416034343698204186575808495617);
-    _2 <- (W256.of_int 4000);
-    tmp370 <@ Primops.mload(_2);
-    _3 <- tmp370;
-    usr_newAggregationChallenge <- (PurePrimops.mulmod usr_curAggregationChallenge _3 _1);
-    _4 <- (W256.of_int 4480);
-    tmp371 <@ usr_pointMulAndAddIntoDest(usr_queriesCommitmentPoint, usr_newAggregationChallenge, _4);
-    tmp372 <@ Primops.mload(usr_valueAtZ);
-    _5 <- tmp372;
-    _6 <- (PurePrimops.mulmod usr_newAggregationChallenge _5 _1);
-    usr_newAggregatedOpeningAtZ <- (PurePrimops.addmod usr_curAggregatedOpeningAtZ _6 _1);
-    return (usr_newAggregationChallenge, usr_newAggregatedOpeningAtZ);
-    }
+  proc low(queriesCommitmentPoint : uint256, valueAtZ : uint256, curAggregationChallenge : uint256, curAggregatedOpeningAtZ : uint256): (uint256 * uint256) = {
+    var newAggregationChallenge, newAggregatedOpeningAtZ, _3, _5, _6;
+    _3 <@ Primops.mload(W256.of_int 4000);
+    newAggregationChallenge <- (PurePrimops.mulmod curAggregationChallenge _3 (W256.of_int Constants.R));
+    PointMulAndAddIntoDest.low(queriesCommitmentPoint, newAggregationChallenge, W256.of_int 4480);
+    _5 <@ Primops.mload(valueAtZ);
+    _6 <- (PurePrimops.mulmod newAggregationChallenge _5 (W256.of_int Constants.R));
+    newAggregatedOpeningAtZ <- (PurePrimops.addmod curAggregatedOpeningAtZ _6 (W256.of_int Constants.R));
+    return (newAggregationChallenge, newAggregatedOpeningAtZ);
+  }
 }.
 
-lemma addAssignRescueCustomGateLinearisationContributionWithV_extracted_equiv_low :
+lemma updateAggregationChallenge_extracted_equiv_low :
     equiv [
-      Verifier_1261.usr_updateAggregationChallenge ~ AddAssignRescueCustomGateLinearisationContributionWithV.low :
-      ={arg, glob AddAssignRescueCustomGateLinearisationContributionWithV} ==>
-      ={res, glob AddAssignRescueCustomGateLinearisationContributionWithV}
+      Verifier_1261.usr_updateAggregationChallenge ~ UpdateAggregationChallenge.low :
+      ={arg, glob UpdateAggregationChallenge} ==>
+      ={res, glob UpdateAggregationChallenge}
     ].
 proof.
   proc.
-  call (pointMulAndAddIntoDest_extracted_equiv_low).
-  inline*. wp. skip. rewrite /Constants.R. by progress.
+  inline Primops.mload. wp.
+  call (pointMulAndAddIntoDest_extracted_equiv_low). wp.
+  skip. rewrite /Constants.R. by progress.
 qed.
